concentration-inequalities/trivialScript.sml
@@ -26,7 +26,42 @@ val UNIV_FUN = store_thm(
 (* Trivial stuff for Reals *)
 (*---------------------------------------------------------------------------*)
 
+val REAL_XOR_LT_GT_EQ = store_thm(
+    "REAL_XOR_LT_GT_EQ",
+    ``∀(x:real) y.
+        ((x = y) ⇒ ¬(x < y) ∧ ¬(y < x)) ∧
+        ((x < y) ⇒ (x ≠ y) ∧ ¬(y < x) ∧ ¬(y ≤ x)) ∧
+        ((x ≤ y) ⇒ ¬(y < x))``,
+    rpt strip_tac >> fs[REAL_LT_GT,REAL_LT_IMP_NE,real_lte]
+);
 
+val ADD_POS = store_thm(
+    "ADD_POS",
+    ``∀x y. ((0:real) ≤ x) ∧ (0 ≤ y) ∧ (x + y = 0) ⇒ (x = 0) ∧ (y = 0)``,
+    rpt strip_tac >> Cases_on `x = 0` >> Cases_on `y = 0` >> fs[] >>
+    `0 < x` by fs[REAL_LT_LE] >> `0 < y` by fs[REAL_LT_LE] >>
+    `0 < x + y` by fs[REAL_LT_ADD] >> fs[REAL_XOR_LT_GT_EQ]
+);
+
+val SUM_GE0 = store_thm(
+    "SUM_GE0",
+    ``∀f n. (∀i. (i < n) ⇒ 0 ≤ f i) ⇒ 0 ≤ sum (0,n) f``,
+    Induct_on `n` >> rpt strip_tac >> fs[sum] >>
+    `0 ≤ sum (0,n) f` by fs[] >> `0 ≤ f n` by fs[] >>
+    fs[REAL_LE_ADD]
+);
+
+val SUM_OF_POS_EQ_0 = store_thm(
+    "SUM_OF_POS_EQ_0",
+    ``∀f n. (sum (0,n) f = 0) ∧ (∀i. (i < n) ⇒ (0 ≤ f i)) ⇒
+        (∀i. (i < n) ⇒ (f i = 0)) ∧ (∀m. (m < n) ⇒ (sum (0,m) f = 0))``,
+    Induct_on `n` >> strip_tac >> fs[sum] >> strip_tac >>
+    `0 ≤ sum (0,n) f` by fs[SUM_GE0] >> `0 ≤ f n` by fs[] >>
+    `(sum (0,n) f = 0) ∧ (f n = 0)` by (strip_tac >> imp_res_tac ADD_POS) >>
+    `(∀i. i < n ⇒ 0 ≤ f i)` by fs[] >> RES_TAC >> rpt strip_tac
+    >- (Cases_on `i = n` >> fs[])
+    >- (Cases_on `m = n` >> fs[])
+);
 
 (*---------------------------------------------------------------------------*)
 (* Trivial stuff for Limits/Derivatives *)
@@ -44,11 +79,55 @@ val DIFF_CADD = store_thm(
 (* Trivial stuff for Extended Reals *)
 (*---------------------------------------------------------------------------*)
 
+val sumfin_def = Define `(sumfin (n,0) f = 0) ∧
+    (sumfin (n,SUC m) f = sumfin (n,m) f + f (n + m))`;
+    
+val prodfin_def = Define `(prodfin (n,0) f = 1) ∧
+    (prodfin (n,SUC m) f = prodfin (n,m) f * f (n + m))`;
+
+val sumfinfun_def = Define `(sumfinfun (n,0) f x = 0) ∧
+    (sumfinfun (n,SUC m) f x = sumfinfun (n,m) f x + f (n + m) x)`;
+    
+val prodfinfun_def = Define `(prodfinfun (n,0) f x = 1) ∧
+    (prodfinfun (n,SUC m) f x = prodfinfun (n,m) f x * f (n + m) x)`;
+
+val closed_interval_def = Define `closed_interval a b = {x | a ≤ x ∧ x ≤ b}`;
+
 val extreal_ln_def = Define
     `(extreal_ln (Normal x) = (if (x ≤ 0) then NegInf else Normal (ln x))) ∧
     (extreal_ln PosInf = PosInf) ∧ (extreal_ln NegInf = NegInf)`;
     
 val _ = overload_on ("ln", Term `extreal_ln`);
+
+val sumfinfun_alt = store_thm(
+    "sumfinfun_alt",
+    ``(∀n f. sumfinfun (n,0) f = (λx. 0)) ∧
+        ∀n m f. sumfinfun (n,SUC m) f = (λx. sumfinfun (n,m) f x + f (n + m) x)``,
+    rpt strip_tac
+    >- (`∀x. sumfinfun (n,0) f x = (λx. 0) x` suffices_by metis_tac[] >>
+        fs[sumfinfun_def])
+    >- (`∀x. sumfinfun (n,SUC m) f x = (λx. sumfinfun (n,m) f x + f (n + m) x) x`
+            suffices_by metis_tac[] >>
+        fs[sumfinfun_def])
+);
+
+val prodfinfun_alt = store_thm(
+    "prodfinfun_alt",
+    ``(∀n f. prodfinfun (n,0) f = (λx. 1)) ∧
+        ∀n m f. prodfinfun (n,SUC m) f = (λx. prodfinfun (n,m) f x * f (n + m) x)``,
+    rpt strip_tac
+    >- (`∀x. prodfinfun (n,0) f x = (λx. 1) x` suffices_by metis_tac[] >>
+        fs[prodfinfun_def])
+    >- (`∀x. prodfinfun (n,SUC m) f x = (λx. prodfinfun (n,m) f x * f (n + m) x) x`
+            suffices_by metis_tac[] >>
+        fs[prodfinfun_def])
+);
+
+val closed_interval_point = store_thm(
+    "closed_interval_point",
+    ``∀y. closed_interval y y = {y}``,
+    strip_tac >> fs[closed_interval_def,EXTENSION,le_antisym]
+);
 
 val extreal_lt_alt = store_thm(
     "extreal_lt_alt",
@@ -57,6 +136,16 @@ val extreal_lt_alt = store_thm(
         (NegInf < Normal r1 ⇔ T) ∧ (Normal r2 < PosInf ⇔ T)``,
     fs[extreal_lt_def,extreal_le_def,real_lte] >>
     Cases_on `b` >> fs[extreal_le_def]
+);
+
+val xor_lt_gt_eq = store_thm(
+    "xor_lt_gt_eq",
+    ``∀(x:extreal) y.
+        ((x = y) ⇒ ¬(x < y) ∧ ¬(y < x)) ∧
+        ((x < y) ⇒ (x ≠ y) ∧ ¬(y < x) ∧ ¬(y ≤ x)) ∧
+        ((x ≤ y) ⇒ ¬(y < x))``,
+    rpt strip_tac >> Cases_on `x` >> Cases_on `y` >> fs[extreal_le_def,extreal_lt_alt] >>
+    fs[REAL_XOR_LT_GT_EQ]
 );
 
 val N0_EQ_0 = store_thm(
@@ -100,6 +189,33 @@ val NORM_REAL_POS1 = store_thm(
     >- (fs[])
 );
 
+val le_mul2 = store_thm(
+    "le_mul2",
+    ``∀x1 x2 y1 y2. (0:extreal) ≤ x1 ∧ 0 ≤ y1 ∧ x1 ≤ x2 ∧ y1 ≤ y2 ⇒ x1 * y1 ≤ x2 * y2``,
+    rpt strip_tac >> `0 ≤ x2` by imp_res_tac le_trans >> `0 ≤ y2` by imp_res_tac le_trans >>
+    `0 = Normal 0` by fs[N0_EQ_0] >> fs[] >> pop_assum kall_tac >>
+    Cases_on `x1` >> Cases_on `y1` >> Cases_on `x2` >> Cases_on `y2` >>
+    fs[extreal_mul_def,extreal_le_def] >> rw[] >> fs[extreal_le_def] >> rw[]
+    >- (metis_tac[REAL_XOR_LT_GT_EQ,real_lte,REAL_LT_LE])
+    >- (metis_tac[REAL_XOR_LT_GT_EQ,real_lte,REAL_LT_LE])
+    >- (metis_tac[REAL_XOR_LT_GT_EQ,real_lte,REAL_LT_LE])
+    >- (metis_tac[REAL_XOR_LT_GT_EQ,real_lte,REAL_LT_LE])
+    >- (metis_tac[REAL_XOR_LT_GT_EQ,real_lte,REAL_LT_LE])
+    >- (metis_tac[REAL_XOR_LT_GT_EQ,real_lte,REAL_LT_LE])
+    >- (`r' = 0` by metis_tac[REAL_LE_ANTISYM] >> fs[])
+    >- (metis_tac[REAL_XOR_LT_GT_EQ,real_lte,REAL_LT_LE])
+    >- (`r = 0` by metis_tac[REAL_LE_ANTISYM] >> fs[])
+    >- (metis_tac[REAL_XOR_LT_GT_EQ,real_lte,REAL_LT_LE])
+    >- (fs[REAL_LE_MUL2])
+);
+
+val sumfin_replace = store_thm(
+    "sumfin_replace",
+    ``∀n f g. (∀i. i < n ⇒ (f i = g i)) ⇒ (sumfin (0,n) f = sumfin (0,n) g)``,
+    Induct_on `n` >> rpt strip_tac >> fs[sumfin_def] >>
+    `sumfin (0,n) f = sumfin (0,n) g` suffices_by (strip_tac >> fs[]) >> fs[]
+);
+
 val EXTR_MUL_CANCEL_LEFT = store_thm(
     "EXTR_MUL_CANCEL_LEFT",
     ``∀x y c. (c ≠ 0) ⇒ ((Normal c * x = Normal c * y) ⇔ (x = y))``,
@@ -127,6 +243,82 @@ val EXTR_MUL_CANCEL_RIGHT = store_thm(
     rpt strip_tac >> eq_tac >> strip_tac >> fs[] >>
     `Normal c * x = Normal c * y` by fs[mul_comm] >>
     imp_res_tac EXTR_MUL_CANCEL_LEFT
+);
+
+val le_lmul_real = store_thm(
+    "le_lmul_real",
+    ``∀x y z. 0 < z ⇒ (x ≤ y ⇔ Normal z * x ≤ Normal z * y)``,
+    rpt strip_tac >> eq_tac >> strip_tac
+    >- (
+        `Normal 0 < Normal z` by fs[extreal_lt_alt] >>
+        fs[N0_EQ_0,le_lt,le_lmul_imp]
+    )
+    >- (
+        `Normal 0 < Normal z` by fs[extreal_lt_alt] >> fs[N0_EQ_0] >>
+        `Normal z ≠ PosInf` by fs[] >>
+        imp_res_tac inv_pos >> `0 < inv (Normal z)` by fs[inv_1over] >>
+        `0 ≤ inv (Normal z)` by fs[lt_le] >>
+        `inv (Normal z) * (Normal z * x) ≤ inv (Normal z) * (Normal z * y)`
+            by imp_res_tac le_lmul_imp >>
+        `z ≠ 0` by fs[REAL_POS_NZ] >>
+        fs[extreal_inv_def,mul_assoc,extreal_mul_def,REAL_MUL_LINV,N1_EQ_1,mul_lone]
+    )
+);
+
+val ext_exp_pos_le = store_thm(
+    "ext_exp_pos_le",
+    ``∀(x:extreal). 0 ≤ exp x``,
+    strip_tac >> `Normal 0 ≤ exp x` suffices_by fs[N0_EQ_0] >>
+    Cases_on `x` >> fs[extreal_exp_def]
+    >- (fs[le_refl])
+    >- (fs[extreal_le_def])
+    >- (fs[extreal_le_def,EXP_POS_LE])
+);
+
+val ext_exp_mono_le = store_thm(
+    "ext_exp_mono_le",
+    ``∀x y. exp x ≤ exp y ⇔ x ≤ y``,
+    rpt strip_tac >> eq_tac >> strip_tac >>
+    Cases_on `x` >> Cases_on `y` >>
+    fs[extreal_le_def,extreal_exp_def,EXP_MONO_LE]
+    >- (fs[EXP_POS_LT,real_lte])
+    >- (fs[EXP_POS_LT,REAL_LT_IMP_LE])
+);
+
+val ext_exp_mono_lt = store_thm(
+    "ext_exp_mono_lt",
+    ``∀x y. exp x < exp y ⇔ x < y``,
+    rpt strip_tac >> eq_tac >> strip_tac >>
+    Cases_on `x` >> Cases_on `y` >>
+    fs[extreal_lt_alt,extreal_exp_def,EXP_MONO_LT]
+    >- ((qspec_then `r` assume_tac) EXP_POS_LT >> metis_tac[REAL_LT_ANTISYM])
+    >- (fs[EXP_POS_LT])
+);
+
+val sumfin_normal = store_thm(
+    "sumfin_normal",
+    ``∀f n. sumfin (0,n) (λi. Normal (f i)) = Normal (sum (0,n) f)``,
+    Induct_on `n` >> rpt strip_tac >> fs[sum,sumfin_def,N0_EQ_0,extreal_add_def]
+);
+
+val prodfin_le = store_thm(
+    "prodfin_le",
+    ``∀f g n. (∀i. i < n ⇒ 0 ≤ f i ∧ f i ≤ g i) ⇒
+        0 ≤ prodfin (0,n) f ∧ prodfin (0,n) f ≤ prodfin (0,n) g``,
+    NTAC 4 strip_tac >> Induct_on `n` >> fs[prodfin_def,le_refl]
+    >- (`Normal 0 ≤ Normal 1` suffices_by fs[N0_EQ_0,N1_EQ_1] >>
+        fs[extreal_le_def])
+    >- (strip_tac >> fs[] >> `0 ≤ f n` by fs[] >> fs[le_mul] >>
+        `f n ≤ g n` by fs[] >> fs[le_mul2])
+);
+
+val exp_sum = store_thm(
+    "exp_sum",
+    ``∀f n. prodfin (0,n) (λi. Normal (exp (f i))) = exp (sumfin (0,n) (λi. Normal (f i)))``,
+    Induct_on `n` >> rpt strip_tac >> fs[prodfin_def,sumfin_def]
+    >- (`Normal 1 = exp (Normal 0)` suffices_by fs[N0_EQ_0,N1_EQ_1] >>
+        fs[extreal_exp_def,EXP_0])
+    >- (fs[sumfin_normal,extreal_exp_def,extreal_mul_def,extreal_add_def,EXP_ADD])
 );
 
 (*---------------------------------------------------------------------------*)
@@ -201,6 +393,24 @@ val IN_MEASURABLE_BOREL_CMUL_ALT = store_thm(
         (qspecl_then [`a`,`f`,`(λx. Normal c * f x)`,`c`] assume_tac) IN_MEASURABLE_BOREL_CMUL >>
         RES_TAC >> fs[]) >>
     fs[]
+);
+
+val IN_MEASURABLE_BOREL_SUMFINFUN = store_thm(
+    "IN_MEASURABLE_BOREL_SUMFINFUN",
+    ``∀a X n. sigma_algebra a ∧ (∀i. i < n ⇒ X i ∈ measurable a Borel) ⇒
+        sumfinfun (0,n) X ∈ measurable a Borel``,
+    rpt strip_tac >> Induct_on `n` >> strip_tac >> fs[] >> rw[]
+    >- (`(λx. 0) ∈ measurable a Borel` by fs[IN_MEASURABLE_BOREL_CONST_ALT] >>
+        `sumfinfun (0,0) X = (λx. 0)` suffices_by fs[] >>
+        `∀x. sumfinfun (0,0) X x = (λx. 0) x` suffices_by metis_tac[] >>
+        strip_tac >> fs[sumfinfun_def])
+    >- (`X n ∈ measurable a Borel` by fs[] >>
+        `(λx. sumfinfun (0,n) X x + X n x) ∈ measurable a Borel`
+            by imp_res_tac IN_MEASURABLE_BOREL_ADD_ALT >>
+        `sumfinfun (0,SUC n) X = (λx. sumfinfun (0,n) X x + X n x)` suffices_by fs[] >>
+        `∀x. sumfinfun (0,SUC n) X x = (λx. sumfinfun (0,n) X x + X n x) x`
+            suffices_by metis_tac[] >>
+        strip_tac >> fs[sumfinfun_def])
 );
 
 (*---------------------------------------------------------------------------*)
@@ -402,9 +612,51 @@ val INT_FN_MINUS_INDIC_LE_FN_MINUS = store_thm(
     )
 );
 
+val integrable_sumfinfun = store_thm(
+    "integrable_sumfinfun",
+    ``∀m n X. (measure_space m) ∧ (∀i. i < n ⇒ integrable m (X i)) ⇒
+        (integrable m (sumfinfun (0,n) X))``,
+    rpt strip_tac >> Induct_on `n` >> fs[sumfinfun_alt,sumfin_def,integrable_zero] >>
+    rpt strip_tac >> fs[] >> `integrable m (X n)` by fs[] >>
+    imp_res_tac integrable_add
+);
+
+val integral_sumfinfun = store_thm(
+    "integral_sumfinfun",
+    ``∀m n X. (measure_space m) ∧ (∀i. i < n ⇒ integrable m (X i)) ⇒
+        (integral m (sumfinfun (0,n) X) = sumfin (0,n) (λi. integral m (X i)))``,
+    rpt strip_tac >> Induct_on `n` >> fs[sumfinfun_alt,sumfin_def,integral_zero] >>
+    rpt strip_tac >> fs[] >> `integrable m (X n)` by fs[] >>
+    `integrable m (sumfinfun (0,n) X)` by fs[integrable_sumfinfun] >>
+    imp_res_tac integral_add >> fs[]
+);
+
 (*---------------------------------------------------------------------------*)
 (* Trivial stuff for Probability *)
 (*---------------------------------------------------------------------------*)
+
+val PROB_SUBSET_PSPACE = store_thm(
+    "PROB_SUBSET_PSPACE",
+    ``∀p s. prob_space p ∧ s ∈ events p ⇒ s ⊆ p_space p``,
+    rpt strip_tac >> fs[prob_space_def,p_space_def,events_def,prob_def] >>
+    fs[MEASURE_SPACE_SUBSET_MSPACE]
+);
+
+val probably_subset = store_thm(
+    "probably_subset",
+    ``∀p s t. prob_space p ∧ probably p s ∧ t ∈ events p ∧ s ⊆ t ⇒ probably p t``,
+    rpt strip_tac >> fs[probably_def] >> imp_res_tac PROB_LE_1 >>
+    imp_res_tac PROB_INCREASING >> rfs[] >> rw[] >> imp_res_tac REAL_LE_ANTISYM
+);
+
+val propably_comp_null = store_thm(
+    "propably_comp_null",
+    ``∀p s. prob_space p ∧ probably p s ⇒ null_set p (p_space p DIFF s)``,
+    rpt strip_tac >> fs[probably_def,null_set_def] >>
+    `p_space p DIFF s ∈ events p ∧ (prob p (p_space p DIFF s) = 0)`
+        suffices_by fs[events_def,prob_def] >>
+    imp_res_tac EVENTS_COMPL >> imp_res_tac PROB_COMPL >> fs[]
+);
 
 val EXPECT_1 = store_thm(
     "EXPECT_1",
@@ -563,6 +815,87 @@ val PSPACE_MBL_IMP_EXP_EQ_EXP_AS = store_thm(
     imp_res_tac INT_FN_MINUS_INDIC_LE_FN_MINUS >>
     pop_assum (qspecl_then [`s`,`f`] assume_tac) >> rfs[] >> fs[extreal_le_def] >>
     NTAC 2 (pop_assum kall_tac)
+);
+
+val probably_inter = store_thm(
+    "probably_inter",
+    ``∀p s t. prob_space p ∧ probably p s ∧ probably p t ⇒ probably p (s ∩ t)``,
+    rpt strip_tac >> fs[probably_def] >> imp_res_tac PROB_COMPL >> rfs[] >>
+    Q.ABBREV_TAC `tc = p_space p DIFF t` >> Q.ABBREV_TAC `sc = p_space p DIFF s` >>
+    imp_res_tac EVENTS_COMPL >> rfs[] >>
+    `(tc ∪ sc) ∈ events p` by imp_res_tac EVENTS_UNION >>
+    `prob p (tc ∪ sc) = 0` by (
+        (qspecl_then [`p`,`(tc ∪ sc)`,`tc`,`sc`] assume_tac) PROB_SUBADDITIVE >>
+        rfs[] >> imp_res_tac PROB_POSITIVE >> imp_res_tac REAL_LE_ANTISYM) >>
+    Q.ABBREV_TAC `tusc = p_space p DIFF (tc ∪ sc)` >>
+    `tusc ∈ events p` by (imp_res_tac EVENTS_COMPL >> rfs[]) >>
+    `prob p tusc = 1` by (imp_res_tac PROB_COMPL >> rfs[]) >>
+    `tusc = s ∩ t` suffices_by (strip_tac >> fs[]) >>
+    Q.UNABBREV_TAC `tusc` >> Q.UNABBREV_TAC `tc` >> Q.UNABBREV_TAC `sc` >>
+    fs[DIFF_DEF,INTER_DEF,UNION_DEF,EXTENSION] >>
+    strip_tac >> EQ_TAC >> strip_tac >> fs[] >>
+    `s ⊆ p_space p` by fs[PROB_SUBSET_PSPACE] >> fs[SUBSET_DEF]
+);
+
+val probably_interval = store_thm(
+    "probably_interval",
+    ``∀p X a b. prob_space p ∧ probably p {x | X x ∈ closed_interval (Normal a) (Normal b)} ⇒ (a ≤ b)``,
+    rpt strip_tac >> Cases_on `a ≤ b` >> fs[] >>
+    fs[prob_space_def,p_space_def,events_def,prob_def,probably_def,closed_interval_def] >>
+    `{x | Normal a ≤ X x ∧ X x ≤ Normal b} = ∅` by (fs[EXTENSION] >> strip_tac >>
+        fs[REAL_NOT_LE] >> `Normal b < Normal a` by fs[extreal_lt_alt] >>
+        Cases_on `Normal a ≤ X x` >> fs[] >> imp_res_tac lte_trans >> fs[extreal_lt_def]) >>
+    imp_res_tac MEASURE_EMPTY >> fs[]
+);
+
+val sumfinfun_probably = store_thm(
+    "sumfinfun_probably",
+    ``∀p n X a. (prob_space p) ∧ (∀i. i < n ⇒ real_random_variable (X i) p) ∧
+        (∀i. i < n ⇒ probably p {x | X i x = Normal (a i)}) ⇒
+        (probably p {x | (sumfinfun (0,n) X x = Normal (sum (0,n) a)) ∧ x ∈ m_space p})``,
+    Induct_on `n` >> rpt strip_tac >> fs[sumfinfun_def,sum]
+    >- (fs[N0_EQ_0] >> rw[] >>
+        fs[prob_space_def,probably_def,p_space_def,events_def,prob_def,MEASURE_SPACE_MSPACE_MEASURABLE])
+    >- (`probably p {x | (sumfinfun (0,n) X x = Normal (sum (0,n) a)) ∧ x ∈ m_space p}`
+            by (RES_TAC >> fs[]) >>
+        `probably p {x | X n x = Normal (a n)}` by fs[] >>
+        `sigma_algebra (m_space p,measurable_sets p)` by fs[prob_space_def,measure_space_def] >>
+        `sumfinfun (0,SUC n) X ∈ measurable (m_space p,measurable_sets p) Borel` by (
+            imp_res_tac IN_MEASURABLE_BOREL_SUMFINFUN >>
+            fs[real_random_variable_def,p_space_def,events_def]) >>
+        qpat_x_assum `∀p X a. _` kall_tac >> NTAC 2 (qpat_x_assum `∀i. _` kall_tac) >>
+        fs[probably_def,events_def,prob_def,sumfinfun_alt] >>
+        `{x | (sumfinfun (0,n) X x + X n x = Normal (sum (0,n) a + a n)) ∧
+            x ∈ m_space p} ∈ measurable_sets p` by (imp_res_tac IN_MEASURABLE_BOREL_ALL >>
+            fs[space_def,subsets_def,INTER_DEF]) >>
+        fs[prob_space_def,p_space_def] >>
+        (qspecl_then [`p`,`{x | X n x = Normal (a n)}`,
+            `{x | (sumfinfun (0,n) X x = Normal (sum (0,n) a)) ∧ x ∈ m_space p}`]
+            assume_tac) MEASURE_SPACE_INTER >>
+        rfs[INTER_DEF] >> Q.ABBREV_TAC `SX = sumfinfun (0,n) X` >> Q.ABBREV_TAC `Sa = sum (0,n) a` >>
+        `measure p {x | (X n x = Normal (a n)) ∧ (SX x = Normal Sa) ∧ x ∈ m_space p} = 1`
+            suffices_by (strip_tac >>
+            `{x | (X n x = Normal (a n)) ∧ (SX x = Normal Sa) ∧ x ∈ m_space p} ⊆
+                {x | (SX x + X n x = Normal (Sa + a n)) ∧ x ∈ m_space p}` by (
+                fs[SUBSET_DEF] >> rpt strip_tac >> fs[extreal_add_def]) >>
+            imp_res_tac MEASURE_SPACE_INCREASING >>
+            (qspecl_then [`p`,
+                `{x | (X n x = Normal (a n)) ∧ (SX x = Normal Sa) ∧ x ∈ m_space p}`,
+                `{x | (SX x + X n x = Normal (Sa + a n)) ∧ x ∈ m_space p}`] assume_tac) INCREASING >>
+            rfs[] >>
+            `measure p {x | (SX x + X n x = Normal (Sa + a n)) ∧ x ∈ m_space p} ≤ 1` by (
+                (qspecl_then [`p`,`{x | (SX x + X n x = Normal (Sa + a n)) ∧ x ∈ m_space p}`]
+                    assume_tac) PROB_LE_1 >>
+                rfs[prob_space_def,p_space_def,events_def,prob_def]) >>
+            imp_res_tac REAL_LE_ANTISYM) >>
+        `{x | (X n x = Normal (a n)) ∧ (SX x = Normal Sa) ∧ x ∈ m_space p} =
+            {x | (SX x = Normal Sa) ∧ x ∈ m_space p} ∩ {x | X n x = Normal (a n)}` by (
+            fs[INTER_DEF,EXTENSION] >> strip_tac >> EQ_TAC >> fs[]) >>
+        fs[] >> pop_assum kall_tac >>
+        (qspecl_then [`p`,`{x | (SX x = Normal Sa) ∧ x ∈ m_space p}`,
+            `{x | X n x = Normal (a n)}`] assume_tac) probably_inter >>
+        rfs[prob_space_def,probably_def,p_space_def,events_def,prob_def]
+    )
 );
 
 val _ = export_theory();
